Added a flag to internal states, drafted a first version of the weak bisimulation over this structure

theories/CTrees.v
@@ -42,7 +42,7 @@ Section ctree.
   Variant ctreeF (ctree : Type) :=
   | RetF (r : R)
   | VisF {X : Type} (e : E X) (k : X -> ctree)
-  | ChoiceF (n : nat) (k : fin n -> ctree)
+  | ChoiceF (vis : bool) (n : nat) (k : fin n -> ctree)
   .
 
   CoInductive ctree : Type := go
@@ -59,7 +59,7 @@ Local Open Scope ctree_scope.
 
 Arguments ctree _ _ : clear implicits.
 Arguments ctreeF _ _ : clear implicits.
-Arguments ChoiceF {_ _} [_] n.
+Arguments ChoiceF {_ _} [_] vis n.
 (* end hide *)
 
 (** A [ctree'] is a "forced" [ctree]. It is the type of inputs
@@ -73,8 +73,10 @@ Definition observe {E R} (t : ctree E R) : ctree' E R := @_observe E R t.
 (** We encode [itree]'s [Tau] constructor as a unary internal choice. *)
 Notation Ret x := (go (RetF x)).
 Notation Vis e k := (go (VisF e k)).
-Notation Tau t := (go (ChoiceF 1 (fun _ => t))).
-Notation Choice n k := (go (ChoiceF n k)).
+Notation Tau t := (go (ChoiceF false 1 (fun _ => t))).
+Notation Choice b n k := (go (ChoiceF b n k)).
+Notation ChoiceV n k := (go (ChoiceF true n k)).
+Notation ChoiceI n k := (go (ChoiceF false n k)).
 
 (** ** Main operations on [ctree] *)
 
@@ -137,7 +139,7 @@ Definition subst {E : Type -> Type} {T U : Type} (k : T -> ctree E U)
     match observe u with
     | RetF r => k r
     | VisF e h => Vis e (fun x => _subst (h x))
-    | ChoiceF n h => Choice n (fun x => _subst (h x))
+    | ChoiceF b n h => Choice b n (fun x => _subst (h x))
     end.
 
 Definition bind {E : Type -> Type} {T U : Type} (u : ctree E T) (k : T -> ctree E U)
@@ -180,7 +182,7 @@ Definition trigger {E : Type -> Type} : E ~> ctree E :=
 
 (** Atomic itrees with choice over a finite arity. *)
 Definition choice {E : Type -> Type} : forall n, ctree E (fin n) :=
-  fun n => Choice n (fun x => Ret x).
+  fun n => ChoiceV n (fun x => Ret x).
 
 (** Ignore the result of a tree. *)
 Definition ignore {E R} : ctree E R -> ctree E unit :=
@@ -189,7 +191,7 @@ Definition ignore {E R} : ctree E R -> ctree E unit :=
 (** Infinite taus. *)
 CoFixpoint spin {E R} : ctree E R := Tau spin.
 CoFixpoint spin_nary {E R} (n : nat) : ctree E R :=
-	Choice n (fun _ => spin_nary n).
+	ChoiceV n (fun _ => spin_nary n).
 
 (** Repeat a computation infinitely. *)
 Definition forever {E R S} (t : ctree E R) : ctree E S :=
@@ -280,7 +282,7 @@ Fixpoint burn (n : nat) {E R} (t : ctree E R) :=
     match observe t with
     | RetF r => Ret r
     | VisF e k => Vis e k
-    | @ChoiceF _ _ _ 1 t' => burn n (t' Fin.F1)
-    | ChoiceF n k => Choice n k
+    | @ChoiceF _ _ _ _ 1 t' => burn n (t' Fin.F1)
+    | ChoiceF b n k => Choice b n k
     end
   end.
