theories/BisimWeak.v
@@ -1,0 +1,129 @@
+(* begin hide *)
+From Coq Require Import
+     Program
+     Setoid
+     Morphisms
+     RelationClasses.
+
+From ITree Require Import
+	Basics.HeterogeneousRelations.
+
+From Coinduction Require Import
+	coinduction rel tactics.
+
+From CTree Require Import
+	Utils CTrees Equ Bisim.
+
+(* end hide *)
+
+Section Internal.
+
+	(* We do not wish to observe internal non-deterministic choices.
+		We therefore want to consider states, i.e. ctrees, that can
+		be reached after a finite number of internal decisions, and
+		are such that they are ready to expose an observation: their
+		head constructor is either a Ret or a Vis.
+		*)
+
+  Context {E : Type -> Type} {R : Type}.
+
+  Inductive internal_ : ctree' E R -> ctree' E R -> Prop :=
+
+  | InternalStep b {n} (x : Fin.t n) k t :
+    		internal_ (observe (k x)) t ->
+    		internal_ (ChoiceF b n k) t
+
+  | InternalStop {n} k k' x :
+    		k x ≅ k' x -> (* Because [internal_] stops right there, we need to close explicitly up to [equ] if we want to be stable under it *)
+    		internal_ (ChoiceF true n k) (observe (k' x)).
+
+  Definition internal u v := internal_ (observe u) (observe v).
+
+  Variant internal_refl : ctree E R -> ctree E R -> Prop :=
+  | InternalRefl : forall u, internal_refl u u 
+  | InternalRel  : forall u v, internal u v -> internal_refl u v.
+
+End Internal.
+
+Section wbisim.
+
+  Context {E : Type -> Type} {R1 R2 : Type} (RR : R1 -> R2 -> Prop).
+
+	(** * [matching]
+	This relation captures the local challenge that two scheduled
+	trees must solve. It corresponds from the more traditional
+	bisimulation world to ensuring that they can take a small step
+	emmitting the same event. *)
+
+  Variant matching' (bisim : ctree E R1 -> ctree E R2 -> Prop) :
+    ctree E R1 -> ctree E R2 -> Prop :=
+  | MatchRet x y (RET : RR x y) :
+     matching' bisim (Ret x) (Ret y)
+  | MatchVis {X} (e : E X) k1 k2 
+     (RET : forall v t', 
+        internal_refl (k1 v) t' ->
+        exists u', internal_refl (k2 v) u' /\ bisim t' u'):
+     matching' bisim (Vis e k1) (Vis e k2)
+  . 
+  Hint Constructors matching': core.
+
+  Variant wbisimF (wbisim : ctree E R1 -> ctree E R2 -> Prop) :
+    ctree E R1 -> ctree E R2 -> Prop :=
+
+  | WBisim u t
+            (SIMFI : forall u', internal u u' ->
+              exists t', internal_refl t t' /\ wbisim u' t')
+            (SIMBI : forall t', internal t t' ->
+              exists u', internal_refl u u' /\ wbisim u' t')
+            (SIMFE : forall u', schedule u u' ->
+              exists t', schedule t t' /\ matching' wbisim u' t')
+            (SIMBE : forall t', schedule t t' ->
+              exists u', schedule u u' /\ matching' wbisim u' t')
+               :
+      wbisimF wbisim u t.
+ 
+  Hint Constructors wbisimF: core.
+(* 
+  Definition wbisim_ eq : ctree E R1 -> ctree E R2 -> Prop :=
+	fun t1 t2 => bisimF eq (observe t1) (observe t2). *)
+
+  Lemma matching'_mono u v sim sim'
+              (IN : matching' sim u v)
+              (LE : sim <= sim') :
+        matching' sim' u v.
+  Proof.
+    inv IN; auto. constructor; intros. edestruct RET as (? & ? & ?); eauto.
+    eexists; split; eauto. 
+    apply LE; auto.
+  Qed.
+  Hint Resolve matching'_mono: core.
+
+  Program Definition fwbisim : mon (ctree E R1 -> ctree E R2 -> Prop) := {| body := wbisimF |}.
+  Next Obligation.
+   unfold pointwise_relation, impl, bisim_.
+   intros ?? INC ?? EQ.
+   constructor; inversion_clear EQ; intros. 
+  - edestruct SIMFI as (? & ? & ?); eauto. 
+  - edestruct SIMBI as (? & ? & ?); eauto. 
+  - edestruct SIMFE as (? & ? & ?); eauto. 
+  - edestruct SIMBE as (? & ? & ?); eauto. 
+  Qed.
+
+End wbisim.
+
+(** associated relation *)
+Definition wbisim {E R} := (gfp (@fbisim E R R eq)).
+(* Notation bisim := (gfp (fbisim eq)). *)
+
+(** associated companions  *)
+Notation T_bis RR  := (t (B (fwbisim RR))).
+Notation t_bis RR  := (t (fwbisim RR)).
+Notation bt_bis RR := (bt (fwbisim RR)).
+
+Infix "≈" := wbisim (at level 70).
+Notation "x ≊ y" := (t_bis eq _ x y) (at level 79).
+Notation "x [≊] y" := (bt_bis eq _ x y) (at level 79).
+
+Arguments wbisim _ _ _ _/.
+#[global] Hint Constructors wbisimF: core.
+#[global] Hint Constructors matching': core.
