theories/Utils.v
@@ -24,3 +24,8 @@ end;
 simpl body in H.
 Tactic Notation "step" "in" ident(H) := step_in H.
 
+Ltac invert := 
+  match goal with 
+  | h : existT _ _ _ = existT _ _ _ |- _ => dependent induction h
+  end.
+
